basic typing execution (no relation for now)

Language.v
@@ -2,6 +2,8 @@ Require Import Coq.Strings.String.
 Require Import Coq.Bool.Bool.
 Require Import Coq.Lists.List.
 Import ListNotations.
+Import StringSyntax.
+Import Ascii.
 
 Module Lang1.
 
@@ -9,16 +11,33 @@ Module Lang1.
 Definition variable : Type := string.
 Definition function : Type := string.
 Inductive type : Type :=
+  | Unit
   | Bool
   | Int
   | String.
   (* | Fun (args : list type) (return_type : type). *)
 
+Definition eqb (tau1 tau2 : type) : bool :=
+  match (tau1, tau2) with
+    | (Bool, Bool) | (Int, Int) | (String, String) => true
+    | _ => false
+  end.
+Notation "tau1 =? tau2" := (eqb tau1 tau2).
+
 (* Value Definition *)
 Inductive value : Type :=
   | UnitValue
   | BoolValue (b : bool)
-  | IntValue (i : nat).
+  | IntValue (i : nat)
+  | StringValue (s : string).
+
+Definition value_to_type (v : value) : type :=
+  match v with
+  | UnitValue => Unit
+  | BoolValue _ => Bool
+  | IntValue _ => Int
+  | StringValue _ => String
+  end.
 
 (* Syntax Definition *)
 Inductive expression : Type :=
@@ -30,118 +49,103 @@ Inductive expression : Type :=
   | Value (v : value).
 
 (* Parsing The Grammar *)
-
-(* Coercion AId : string >-> aexp. *)
-(* Coercion ANum : nat >-> aexp. *)
+Coercion IntValue : nat >-> value.
+Coercion StringValue : string >-> value.
+Coercion Value : value >-> expression.
 
 Declare Custom Entry com.
 Declare Scope com_scope.
 Declare Custom Entry com_aux.
 
-
 Notation "<{ e }>" := e (e custom com_aux) : com_scope.
 Notation "e" := e (in custom com_aux at level 0, e custom com) : com_scope.
 Notation "( x )" := x (in custom com, x at level 99) : com_scope.
-
 Notation "x" := x (in custom com at level 0, x constr at level 0) : com_scope.
-Notation "f x .. y" := (.. (f x) .. y)
-                  (in custom com at level 0, only parsing,
-                  f constr at level 0, x constr at level 9,
-                  y constr at level 9) : com_scope.
-(* Notation "x + y"   := (APlus x y) (in custom com at level 50, left associativity). *)
-(* Notation "x - y"   := (AMinus x y) (in custom com at level 50, left associativity). *)
-(* Notation "x * y"   := (AMult x y) (in custom com at level 40, left associativity). *)
-(* Notation "'true'"  := true (at level 1). *)
-(* Notation "'true'"  := BTrue (in custom com at level 0). *)
-(* Notation "'false'" := false (at level 1). *)
-(* Notation "'false'" := BFalse (in custom com at level 0). *)
-(* Notation "x <= y"  := (BLe x y) (in custom com at level 70, no associativity). *)
-(* Notation "x > y"   := (BGt x y) (in custom com at level 70, no associativity). *)
-(* Notation "x = y"   := (BEq x y) (in custom com at level 70, no associativity). *)
-(* Notation "x <> y"  := (BNeq x y) (in custom com at level 70, no associativity). *)
-(* Notation "x && y"  := (BAnd x y) (in custom com at level 80, left associativity). *)
-(* Notation "'~' b"   := (BNot b) (in custom com at level 75, right associativity). *)
-(* Notation "'skip'"  := *)
-(*          CSkip (in custom com at level 0) : com_scope. *)
-
-
+Notation "f x .. y " := (.. (f x) .. y)
+  (in custom com at level 0, only parsing,
+  f constr at level 0, 
+  x constr at level 10, (* level of x and y should be the same *)
+  y constr at level 10) : com_scope.
 Notation "()" := (Value UnitValue)(in custom com at level 0) : com_scope.
 Notation "'let' x = e1 ; e2"  :=
-         (Let x e1 e2)
-            (in custom com at level 0, x constr at level 0,
-             e1 at level 85, no associativity) : com_scope.
+  (Let x e1 e2)
+  (in custom com at level 0,
+  x constr at level 0,
+  e1 constr at level 0,
+  e2 at level 90,
+  right associativity) : com_scope.
 Notation "x = y"  :=
-         (Assign x y)
-            (in custom com at level 0, x constr at level 0,
-             y at level 85, no associativity) : com_scope.
+  (Assign x y)
+  (in custom com at level 0,
+  x constr at level 0,
+  y at level 70,
+  no associativity) : com_scope.
 Notation "x ; y" :=
-         (Sequence x y)
-           (in custom com at level 90,
-            right associativity) : com_scope.
-(* Notation "'if' x 'then' y 'else' z 'end'" := *)
-(*          (CIf x y z) *)
-(*            (in custom com at level 89, x at level 99, *)
-(*             y at level 99, z at level 99) : com_scope. *)
-(* Notation "'while' x 'do' y 'end'" := *)
-(*          (CWhile x y) *)
-(*            (in custom com at level 89, x at level 99, *)
-(*             y at level 99) : com_scope. *)
-
-(* Notation "e1 ';' e2" := (Sequence e1 e2)(at level 60). *)
-(* Notation "'let' x = e1 ; e2" := (Let x e1 e2)(at level 70). *)
-(* (* Notation "f ( e1 ... e2 ") *) *)
-(* Notation "x '=' e" := (Assign x e). *)
+  (Sequence x y)
+  (in custom com at level 80,
+  right associativity) : com_scope.
 
 Open Scope com_scope.
 
-(* Test Syntax Notation *)
-Lemma test1 : forall (e1 e2 : expression),
-  <{ e1 ; e2 }> = Sequence e1 e2.
+(* Test Syntax Notation *) (* Unset Printing Notations *)
+Lemma test1 : forall (e1 e2 : expression), <{ e1 ; e2 }> = Sequence e1 e2.
 Proof. reflexivity. Qed.
-Lemma test2 : forall (e : expression) (x : variable),
-  <{ x = e }> = Assign x e.
+Lemma test2 : forall (e : expression) (x : variable), <{ x = e }> = Assign x e.
 Proof. reflexivity. Qed.
 Lemma test3 : forall (e : expression) (x : variable),
   <{ x = e ; Var x }> = Sequence (Assign x e) (Var x).
 Proof. reflexivity. Qed.
-Lemma test4 : forall (e : expression) (x : variable), 
-  <{ let x = e ;  x = e }> = Let x e (Assign x e). 
+Lemma test4 : forall (e : expression) (x : variable),
+  <{ let x = e ;  x = e }> = Let x e (Assign x e).
 Proof. reflexivity. Qed.
-Lemma test5 : forall (e : expression) (x : variable), 
-  <{ x = e ; let x = e ; () }> = Sequence (Assign x e) (Let x e (Value UnitValue)). 
+Lemma test5 : forall (e : expression) (x : variable),
+  <{ x = e ; let x = e ; () }> 
+    = Sequence (Assign x e) (Let x e (Value UnitValue)).
 Proof. reflexivity. Qed.
 Lemma test6 : forall (e : expression) (x : variable), 
   <{ x = e }> = Assign x e.
 Proof. reflexivity. Qed.
 Lemma test7 : forall (e1 e2 : expression) (x y : variable), 
-  <{
-    let x = e1 ;
-    let y = e2 ;
-    ()
-  }> = Let x e1 (Let y e2 (Value UnitValue)).
+  <{ let x = e1 ; let y = e2 ; () }> 
+  = Let x e1 (Let y e2 (Value UnitValue)).
+Proof. reflexivity. Qed.
+Lemma test8 : forall (x : variable) (e : expression),
+  <{ let x = 4 ; e }> = Let x 4 e.
+Proof. reflexivity. Qed.
+Lemma test9 : forall (e1 e2 e3 : expression),
+  <{ e1; e2; e3 }> = Sequence e1 (Sequence e2 e3).
+Proof. reflexivity. Qed.
+Lemma test10 : forall (x y z : variable),
+  <{let x = 2; let y = 3; let z = 4; ()}> = Let x 2 (Let y 3 (Let z 4 <{()}>)).
+Proof. reflexivity. Qed.
+Lemma test11 : forall (x y : variable) (e : expression),
+  <{ x = 8; x ; let y = 4 ; x }> 
+    = Sequence (Assign x 8) (Sequence x (Let y 4 x)).
+Proof. reflexivity. Qed.
+Lemma test12 : forall (x : variable) (e : expression),
+  <{ let x = 4; x = 8; e }> = Let x 4 (Sequence (Assign x 8) e).
 Proof. reflexivity. Qed.
 
 (* Typing Relation Definition *)
-Definition typingEnv : Type := list (variable * type).
+Inductive refinement : Type := 
+  | None
+  | NotAccessible.
+Definition refined_type : Type := refinement * type.
+Definition typingEnv : Type := list (variable * refined_type).
 (* Reserved Notation "Gamma '|-' x ':' tau" (at level 100). *)
 
-Inductive type_of : typingEnv -> variable -> type -> Prop :=
+Inductive type_expression : typingEnv -> variable -> type -> Prop :=
   | Env_Empty (x : variable) (tau : type) :
-      type_of [(x, tau)] x tau
+      type_expression [(x, (None, tau))] x tau
   | Env_Rec (gamma : typingEnv) (x y : variable) (taux tauy : type) :
       x <> y
-      -> type_of ((y, tauy)::gamma) x taux
-      -> type_of gamma x taux.
-        (* where "gamma '|-' x ':' tau" := (typing gamma x tau) : type_scope. *)
+      -> type_expression ((y, (None, tauy))::gamma) x taux
+      -> type_expression gamma x taux.
+(* where "gamma '|-' x ':' tau" := (typing gamma x tau) : type_scope. *)
 
 Lemma test50 : forall (x : variable) (tau : type),
-  (type_of [(x, tau)] x tau).
+  (type_expression [(x, (None, tau))] x tau).
 Proof. apply Env_Empty. Qed.
-
-Import StringSyntax.
-Import Ascii.
-Search "eqb".
-(* Search "String.eqb". *)
 
 Inductive result (A E: Type) : Type :=
 | Ok (x : A)
@@ -151,19 +155,25 @@ Arguments Ok [A E].
 Arguments Error [A E].
 
 Inductive customError : Type :=
-  | TypeError
   | ExecutionError
-  | NonTerminatingFixpoint
+  | NonTerminatingFunction
   | Todo
-  | VariableNotTypable.
+  | VariableNotTypable
+  | TypeError (expected given : type).
 
+
+(* Function Typing Variable *)
 Fixpoint typing_var_exec
-  (gamma : typingEnv) (x : variable) : (result type customError) :=
+  (gamma : typingEnv) (x : variable) : (result (type * typingEnv) customError) :=
     match gamma with
     | [] => Error VariableNotTypable
-    | (y , tau)::gamma' =>
+    | (y , (_, tau))::gamma' =>
         if (String.eqb x y)
-        then Ok tau
+        then
+          match tau with
+          | Unit | Bool | Int => Ok (tau, gamma)
+          | String => Ok (tau, (y, (NotAccessible, tau))::gamma')
+          end
         else (typing_var_exec gamma' x)
   end.
 
@@ -172,34 +182,79 @@ Lemma test100 : forall (x : variable),
 Proof. reflexivity. Qed.
 Lemma test101 : forall (x y : variable),
   String.eqb x y = true ->
-  typing_var_exec [(y, Int)] x = Ok Int.
+  typing_var_exec [(y, (None, Int))] x = Ok (Int, [(y, (None, Int))]).
 Proof. intros. simpl. rewrite H. reflexivity. Qed.
-
 Lemma test102 : forall (x : variable),
   typing_var_exec [] x = Error VariableNotTypable.
 Proof. reflexivity. Qed.
 
-Fixpoint typing_expr_exec
+(* Function Typing Expression *)
+Fixpoint typing_expression_exec
   (n : nat) (gamma : typingEnv) (e : expression)
   : (result (type * typingEnv) customError) :=
   match n with
-  | 0 => Error NonTerminatingFixpoint
+  | 0 => Error NonTerminatingFunction
   | S i =>
-      match e with
-      | Sequence e1 e2 =>
-          match typing_expr_exec i gamma e1 with
+  match e with
+  | <{ e1 ; e2 }> =>
+      match typing_expression_exec i gamma e1 with
+      | Error err => Error err
+      | Ok (tau1, gamma1) =>
+          match typing_expression_exec i gamma1 e2 with
           | Error err => Error err
-          | Ok (tau1, gamma1) =>
-              match typing_expr_exec i gamma1 e2 with
-              | Error err => Error err
-              | Ok (gamma2, tau2) => Error Todo
-              end
+          | Ok (tau2, gamma2) =>
+              if (tau1 =? Unit)
+              then Ok (tau2, gamma2)
+              else Error (TypeError Unit tau1)
           end
-      | _ => Error Todo
       end
+  | <{ let x = e1 ; e2 }> =>
+      match typing_expression_exec i gamma e1 with
+      | Ok (tau1, gamma1) =>
+          typing_expression_exec i ((x, (None, tau1))::gamma1) e2
+      | err => err
+      end
+  | Var x =>
+    match typing_var_exec gamma x with
+    | Error err => Error err
+    | Ok (tau, gamma') => Ok (tau, gamma') (* TODO get different gamma borrow checking *)
+    end
+  | Value v => Ok (value_to_type v, gamma)
+  | <{ x = e }> =>
+    match typing_expression_exec i gamma e with
+    | Error err => Error err
+    | Ok (tau, gamma') => Error Todo
+    end
+  | _ => Error Todo
+  end
   end.
 
+(* BigInt use for making sure function terminates *)
+Definition BigNat := 10000.
+(* Check BigNat. *)
+
+Lemma test150 : forall (x : variable),
+  typing_expression_exec BigNat [] <{ 4128 }> = Ok (Int, []).
+Proof. intros. simpl. reflexivity. Qed.
+Lemma test151 : forall (x : variable),
+  typing_expression_exec BigNat [] <{ let x = 4128 ; Var x }>
+    = Ok (Int, [(x, (None, Int))]).
+Proof. intros. simpl. rewrite String.eqb_refl. reflexivity. Qed.
+Lemma test152 : forall (x : variable) (s : string),
+  typing_expression_exec BigNat [] <{ let x = s ; Var x }> 
+    = Ok (String, [(x, (NotAccessible, String))]).
+Proof. intros. simpl. rewrite String.eqb_refl. reflexivity. Qed.
+
+Fixpoint semantics_exec 
+  (n : nat) (e : expression) : result value customError :=
+  match n with
+  | 0 => Error NonTerminatingFunction
+  | S i => 
+  match e with
+  | _ => Error Todo
+  end
+  end
+.
+
+
 End Lang1.
-
-
-
